src/opt/Compatibility.v
@@ -17,313 +17,18 @@ Require Import Memory.
 Require Import Commit.
 Require Import Thread.
 Require Import Configuration.
-Require Import Simulation.
+
 Require Import FulfillStep.
-Require Import MemInv.
+Require Import SimMemory.
+Require Import SimPromises.
+Require Import SimLocal.
+Require Import Simulation.
 
 Require Import Syntax.
 Require Import Semantics.
 
 Set Implicit Arguments.
 
-
-Lemma sim_local_cell_bot
-      loc lc_src lc_tgt
-      (SIM: sim_local lc_src lc_tgt)
-      (BOT: lc_tgt.(Local.promises) loc = Cell.bot):
-  lc_src.(Local.promises) loc = Cell.bot.
-Proof.
-  inv SIM. eapply MemInv.sem_bot_inv in PROMISES; auto. rewrite PROMISES. auto.
-Qed.
-
-Lemma sim_local_memory_bot
-      lc_src lc_tgt
-      (SIM: sim_local lc_src lc_tgt)
-      (BOT: lc_tgt.(Local.promises) = Memory.bot):
-  lc_src.(Local.promises) = Memory.bot.
-Proof.
-  inv SIM. eapply MemInv.sem_bot_inv in PROMISES; auto. rewrite PROMISES. auto.
-Qed.
-
-Lemma sim_local_future
-      inv
-      lc_src mem1_src mem2_src
-      lc_tgt mem1_tgt
-      (INV1: MemInv.sem inv lc_src.(Local.promises) lc_tgt.(Local.promises))
-      (LE1: Memory.le lc_tgt.(Local.promises) lc_src.(Local.promises))
-      (MEM1: Memory.sim mem1_tgt mem1_src)
-      (FUTURE_SRC: Memory.future mem1_src mem2_src)
-      (WF1_SRC: Local.wf lc_src mem1_src)
-      (WF1_TGT: Local.wf lc_tgt mem1_tgt)
-      (WF2_SRC: Local.wf lc_src mem2_src)
-      (MEM2_SRC: Memory.closed mem2_src):
-  exists mem2_tgt,
-    <<MEM2: Memory.sim mem2_tgt mem2_src>> /\
-    <<FUTURE_TGT: Memory.future mem1_tgt mem2_tgt>> /\
-    <<WF2_TGT: Local.wf lc_tgt mem2_tgt>> /\
-    <<MEM2_TGT: Memory.closed mem2_tgt>>.
-Proof.
-  esplits.
-  - reflexivity.
-  - etrans; eauto. apply Memory.sim_future. apply MEM1.
-  - econs.
-    + apply WF1_TGT.
-    + eapply Commit.future_closed; try apply WF1_TGT; eauto.
-      etrans; eauto. apply Memory.sim_future. apply MEM1.
-    + etrans; eauto. apply WF2_SRC.
-  - auto.
-Qed.
-
-Lemma sim_local_promise
-      lc1_src mem1_src
-      lc1_tgt mem1_tgt
-      lc2_tgt mem2_tgt
-      loc from to val released kind
-      (STEP_TGT: Local.promise_step lc1_tgt mem1_tgt loc from to val released lc2_tgt mem2_tgt kind)
-      (LOCAL1: sim_local lc1_src lc1_tgt)
-      (MEM1: Memory.sim mem1_tgt mem1_src)
-      (WF1_SRC: Local.wf lc1_src mem1_src)
-      (WF1_TGT: Local.wf lc1_tgt mem1_tgt)
-      (MEM1_SRC: Memory.closed mem1_src)
-      (MEM1_TGT: Memory.closed mem1_tgt):
-  exists lc2_src mem2_src,
-    <<STEP_SRC: Local.promise_step lc1_src mem1_src loc from to val released lc2_src mem2_src kind>> /\
-    <<LOCAL2: sim_local lc2_src lc2_tgt>> /\
-    <<MEM2: Memory.sim mem2_tgt mem2_src>>.
-Proof.
-  inv LOCAL1. inv STEP_TGT.
-  exploit MemInv.promise; eauto.
-  { apply WF1_SRC. }
-  { apply WF1_TGT. }
-  i. des.
-  exploit Memory.future_closed_capability; eauto.
-  { apply Memory.sim_future. eauto. }
-  i. des.
-  exploit Memory.promise_future; try apply PROMISE_SRC; eauto.
-  { apply WF1_SRC. }
-  i. des.
-  esplits; eauto.
-  - econs; eauto.
-  - econs; eauto.
-Qed.
-
-Lemma sim_local_read
-      lc1_src mem1_src
-      lc1_tgt mem1_tgt
-      lc2_tgt
-      loc ts val released_tgt ord_src ord_tgt
-      (STEP_TGT: Local.read_step lc1_tgt mem1_tgt loc ts val released_tgt ord_tgt lc2_tgt)
-      (LOCAL1: sim_local lc1_src lc1_tgt)
-      (MEM1: Memory.sim mem1_tgt mem1_src)
-      (WF1_SRC: Local.wf lc1_src mem1_src)
-      (WF1_TGT: Local.wf lc1_tgt mem1_tgt)
-      (MEM1_SRC: Memory.closed mem1_src)
-      (MEM1_TGT: Memory.closed mem1_tgt)
-      (ORD: Ordering.le ord_src ord_tgt):
-  exists released_src lc2_src,
-    <<REL: Capability.le released_src released_tgt>> /\
-    <<STEP_SRC: Local.read_step lc1_src mem1_src loc ts val released_src ord_src lc2_src>> /\
-    <<LOCAL2: sim_local lc2_src lc2_tgt>>.
-Proof.
-  inv LOCAL1. inv STEP_TGT.
-  exploit Memory.sim_get; try apply MEM1; eauto. i. des.
-  esplits; eauto.
-  - econs; eauto. eapply CommitFacts.readable_mon; eauto.
-  - econs; eauto. s. apply CommitFacts.read_commit_mon; auto.
-    + apply WF1_TGT.
-    + eapply MEM1_TGT. eauto.
-Qed.
-
-Lemma sim_local_fulfill
-      lc1_src sc1_src mem1_src
-      lc1_tgt sc1_tgt mem1_tgt
-      lc2_tgt sc2_tgt
-      loc from to val releasedm_src releasedm_tgt released ord
-      (RELM_LE: Capability.le releasedm_src releasedm_tgt)
-      (RELM_WF: Capability.wf releasedm_src)
-      (RELM_CLOSED: Memory.closed_capability releasedm_src mem1_src)
-      (WF_RELM_TGT: Capability.wf releasedm_tgt)
-      (STEP_TGT: fulfill_step lc1_tgt sc1_tgt loc from to val releasedm_tgt released ord lc2_tgt sc2_tgt)
-      (LOCAL1: sim_local lc1_src lc1_tgt)
-      (SC1: TimeMap.le sc1_src sc1_tgt)
-      (MEM1: Memory.sim mem1_tgt mem1_src)
-      (WF1_SRC: Local.wf lc1_src mem1_src)
-      (WF1_TGT: Local.wf lc1_tgt mem1_tgt)
-      (SC1_SRC: Memory.closed_timemap sc1_src mem1_src)
-      (SC1_TGT: Memory.closed_timemap sc1_tgt mem1_tgt)
-      (MEM1_SRC: Memory.closed mem1_src)
-      (MEM1_TGT: Memory.closed mem1_tgt):
-  exists lc2_src sc2_src,
-    <<STEP_SRC: fulfill_step lc1_src sc1_src loc from to val releasedm_src released ord lc2_src sc2_src>> /\
-    <<LOCAL2: sim_local lc2_src lc2_tgt>> /\
-    <<SC2: TimeMap.le sc2_src sc2_tgt>>.
-Proof.
-  inv STEP_TGT.
-  assert (RELT_LE:
-   Capability.le
-     (Capability.join releasedm_src
-        (Commit.rel
-           (Commit.write_commit (Local.commit lc1_src) sc1_src loc to
-              ord) loc))
-     (Capability.join releasedm_tgt
-        (Commit.rel
-           (Commit.write_commit (Local.commit lc1_tgt) sc1_tgt loc to
-              ord) loc))).
-  { committac.
-    - etrans; eauto. committac.
-    - rewrite <- Capability.join_r.
-      rewrite <- Capability.join_l.
-      apply LOCAL1.
-    - condtac; committac; try apply WF1_TGT.
-      + rewrite <- Capability.join_r.
-        rewrite <- Capability.join_r.
-        rewrite <- Capability.join_l.
-        rewrite <- Capability.join_l.
-        apply LOCAL1.
-      + condtac; committac.
-      + etrans; [|apply TimeMap.join_r].
-        etrans; [|apply TimeMap.join_r].
-        etrans; [|apply TimeMap.join_l].
-        etrans; [|apply TimeMap.join_r].
-        unfold TimeMap.singleton, LocFun.add. condtac; [refl|congr].
-      + condtac; committac.
-        rewrite <- Capability.join_r.
-        rewrite <- Capability.join_r.
-        rewrite <- Capability.join_r.
-        econs; try refl. ss.
-  }
-  assert (RELT_WF:
-   Capability.wf
-     (Capability.join releasedm_src
-        (Commit.rel
-           (Commit.write_commit (Local.commit lc1_src) sc1_src loc to
-              ord) loc))).
-  { repeat (try condtac; committac; try apply WF1_SRC). }
-  exploit MemInv.remove; try exact REMOVE; eauto.
-  { apply LOCAL1. }
-  { apply LOCAL1. }
-  { apply WF1_SRC. }
-  { apply WF1_TGT. }
-  i. des. esplits.
-  - econs; eauto.
-    + etrans; eauto.
-    + eapply CommitFacts.writable_mon; eauto. apply LOCAL1. refl.
-  - econs; eauto. s. apply CommitFacts.write_commit_mon; auto.
-    + apply LOCAL1.
-    + apply WF1_TGT.
-    + refl.
-  - apply CommitFacts.write_sc_mon; auto. refl.
-Qed.
-
-Lemma sim_local_write
-      lc1_src sc1_src mem1_src
-      lc1_tgt sc1_tgt mem1_tgt
-      lc2_tgt sc2_tgt mem2_tgt
-      loc from to val releasedm_src releasedm_tgt released_tgt ord kind
-      (RELM_LE: Capability.le releasedm_src releasedm_tgt)
-      (RELM_SRC_WF: Capability.wf releasedm_src)
-      (RELM_SRC_CLOSED: Memory.closed_capability releasedm_src mem1_src)
-      (RELM_TGT_WF: Capability.wf releasedm_tgt)
-      (RELM_TGT_CLOSED: Memory.closed_capability releasedm_tgt mem1_tgt)
-      (STEP_TGT: Local.write_step lc1_tgt sc1_tgt mem1_tgt loc from to val releasedm_tgt released_tgt ord lc2_tgt sc2_tgt mem2_tgt kind)
-      (LOCAL1: sim_local lc1_src lc1_tgt)
-      (SC1: TimeMap.le sc1_src sc1_tgt)
-      (MEM1: Memory.sim mem1_tgt mem1_src)
-      (WF1_SRC: Local.wf lc1_src mem1_src)
-      (WF1_TGT: Local.wf lc1_tgt mem1_tgt)
-      (SC1_SRC: Memory.closed_timemap sc1_src mem1_src)
-      (SC1_TGT: Memory.closed_timemap sc1_tgt mem1_tgt)
-      (MEM1_SRC: Memory.closed mem1_src)
-      (MEM1_TGT: Memory.closed mem1_tgt):
-  exists released_src lc2_src sc2_src mem2_src,
-    <<STEP_SRC: Local.write_step lc1_src sc1_src mem1_src loc from to val releasedm_src released_src ord lc2_src sc2_src mem2_src kind>> /\
-    <<REL2: Capability.le released_src released_tgt>> /\
-    <<LOCAL2: sim_local lc2_src lc2_tgt>> /\
-    <<SC2: TimeMap.le sc2_src sc2_tgt>> /\
-    <<MEM2: Memory.sim mem2_tgt mem2_src>>.
-Proof.
-  exploit write_promise_fulfill; eauto. i. des.
-  exploit Local.promise_step_future; eauto. i. des.
-  exploit sim_local_promise; eauto. i. des.
-  exploit Local.promise_step_future; eauto. i. des.
-  exploit sim_local_fulfill; try apply STEP2;
-    try apply LOCAL2; try apply MEM2; eauto.
-  { eapply Memory.future_closed_capability; eauto. }
-  i. des.
-  exploit promise_fulfill_write; try exact STEP_SRC; try exact STEP_SRC0; eauto.
-  { i. exploit ORD; eauto. i. des.
-    splits; auto. eapply sim_local_cell_bot; eauto.
-  }
-  i. des. esplits; eauto. etrans; eauto.
-Qed.
-
-Lemma sim_local_update
-      lc1_src sc1_src mem1_src
-      lc1_tgt sc1_tgt mem1_tgt
-      lc2_tgt
-      lc3_tgt sc3_tgt mem3_tgt
-      loc ts1 val1 released1_tgt ord1_src ord1_tgt
-      from2 to2 val2 released2_tgt ord2 kind
-      (STEP1_TGT: Local.read_step lc1_tgt mem1_tgt loc ts1 val1 released1_tgt ord1_tgt lc2_tgt)
-      (STEP2_TGT: Local.write_step lc2_tgt sc1_tgt mem1_tgt loc from2 to2 val2 released1_tgt released2_tgt ord2 lc3_tgt sc3_tgt mem3_tgt kind)
-      (LOCAL1: sim_local lc1_src lc1_tgt)
-      (SC1: TimeMap.le sc1_src sc1_tgt)
-      (MEM1: Memory.sim mem1_tgt mem1_src)
-      (WF1_SRC: Local.wf lc1_src mem1_src)
-      (WF1_TGT: Local.wf lc1_tgt mem1_tgt)
-      (SC1_SRC: Memory.closed_timemap sc1_src mem1_src)
-      (SC1_TGT: Memory.closed_timemap sc1_tgt mem1_tgt)
-      (MEM1_SRC: Memory.closed mem1_src)
-      (MEM1_TGT: Memory.closed mem1_tgt)
-      (ORD: Ordering.le ord1_src ord1_tgt):
-  exists released1_src released2_src lc2_src lc3_src sc3_src mem3_src,
-    <<REL1: Capability.le released1_src released1_tgt>> /\
-    <<REL2: Capability.le released2_src released2_tgt>> /\
-    <<STEP1_SRC: Local.read_step lc1_src mem1_src loc ts1 val1 released1_src ord1_src lc2_src>> /\
-    <<STEP2_SRC: Local.write_step lc2_src sc1_src mem1_src loc from2 to2 val2 released1_src released2_src ord2 lc3_src sc3_src mem3_src kind>> /\
-    <<LOCAL3: sim_local lc3_src lc3_tgt>> /\
-    <<SC3: TimeMap.le sc3_src sc3_tgt>> /\
-    <<MEM3: Memory.sim mem3_tgt mem3_src>>.
-Proof.
-  exploit Local.read_step_future; eauto. i. des.
-  exploit sim_local_read; eauto. i. des.
-  exploit Local.read_step_future; eauto. i. des.
-  exploit sim_local_write; eauto. i. des.
-  esplits; eauto.
-Qed.
-
-Lemma sim_local_fence
-      lc1_src sc1_src mem1_src
-      lc1_tgt sc1_tgt mem1_tgt
-      lc2_tgt sc2_tgt
-      ordr_src ordw_src
-      ordr_tgt ordw_tgt
-      (STEP_TGT: Local.fence_step lc1_tgt sc1_tgt mem1_tgt ordr_tgt ordw_tgt lc2_tgt sc2_tgt)
-      (LOCAL1: sim_local lc1_src lc1_tgt)
-      (SC1: TimeMap.le sc1_src sc1_tgt)
-      (MEM1: Memory.sim mem1_tgt mem1_src)
-      (WF1_SRC: Local.wf lc1_src mem1_src)
-      (WF1_TGT: Local.wf lc1_tgt mem1_tgt)
-      (ORDR: Ordering.le ordr_src ordr_tgt)
-      (ORDW: Ordering.le ordw_src ordw_tgt):
-  exists lc2_src sc2_src,
-    <<STEP_SRC: Local.fence_step lc1_src sc1_src mem1_src ordr_src ordw_src lc2_src sc2_src>> /\
-    <<LOCAL2: sim_local lc2_src lc2_tgt>> /\
-    <<SC2: TimeMap.le sc2_src sc2_tgt>>.
-Proof.
-  inv STEP_TGT. esplits; eauto.
-  - econs; eauto. i. eapply sim_local_memory_bot; eauto.
-    apply RELEASE. etrans; eauto.
-  - econs; try apply LOCAL1. s.
-    apply CommitFacts.write_fence_commit_mon; auto; try refl.
-    apply CommitFacts.read_fence_commit_mon; auto; try refl.
-    + apply LOCAL1.
-    + apply WF1_TGT.
-  - apply CommitFacts.write_fence_sc_mon; auto; try refl.
-    apply CommitFacts.read_fence_commit_mon; auto; try refl.
-    + apply LOCAL1.
-    + apply WF1_TGT.
-Qed.
 
 Definition SIM_REGS := forall (rs_src rs_tgt:RegFile.t), Prop.
 
@@ -625,7 +330,7 @@ Proof.
     apply rclo9_incl.
   - (* nil *)
     ii.
-    inversion LOCAL. apply MemInv.sem_bot_inv in PROMISES; auto.
+    inversion LOCAL. apply SimPromises.sem_bot_inv in PROMISES; auto.
     destruct lc_src, lc_tgt. ss. subst.
     splits; s; ii.
     { inv TERMINAL_TGT. ss. esplits; eauto; ss. }
@@ -633,7 +338,7 @@ Proof.
       esplits; eauto.
       - etrans.
         + apply Memory.max_timemap_spec; eauto. committac.
-        + apply Memory.sim_max_timemap; eauto. committac.
+        + apply sim_memory_max_timemap; eauto.
       - etrans.
         + apply Memory.max_timemap_spec; eauto. committac.
         + apply Memory.future_max_timemap; eauto.
@@ -652,7 +357,7 @@ Proof.
     + apply rclo9_step. apply ctx_nil; auto.
   - (* instr *)
     ii.
-    inversion LOCAL. apply MemInv.sem_bot_inv in PROMISES; auto.
+    inversion LOCAL. apply SimPromises.sem_bot_inv in PROMISES; auto.
     destruct lc_src, lc_tgt. ss. subst.
     splits; s; ii.
     { inv TERMINAL_TGT. }
@@ -660,7 +365,7 @@ Proof.
       esplits; eauto.
       - etrans.
         + apply Memory.max_timemap_spec; eauto. committac.
-        + apply Memory.sim_max_timemap; eauto. committac.
+        + apply sim_memory_max_timemap; eauto.
       - etrans.
         + apply Memory.max_timemap_spec; eauto. committac.
         + apply Memory.future_max_timemap; eauto.
@@ -732,7 +437,7 @@ Proof.
     splits; s; ii.
     { inv TERMINAL_TGT. destruct stmts1_tgt, stmts2_tgt; inv H0.
       exploit TERMINAL; try by econs. i. des.
-      inversion LOCAL. exploit MemInv.sem_bot_inv; eauto. i.
+      inversion LOCAL. exploit SimPromises.sem_bot_inv; eauto. i.
       destruct lc2_src. ss. subst.
       destruct st2_src. inv TERMINAL_SRC. ss. subst.
       exploit Thread.rtc_step_future; eauto. s. i. des.
@@ -755,7 +460,7 @@ Proof.
     }
     destruct stmts1_tgt.
     + exploit TERMINAL; try by econs. i. des.
-      inversion LOCAL. exploit MemInv.sem_bot_inv; eauto. i. subst.
+      inversion LOCAL. exploit SimPromises.sem_bot_inv; eauto. i. subst.
       destruct st2_src, lc2_src. inv TERMINAL_SRC. ss. subst.
       exploit Thread.rtc_step_future; eauto. s. i. des.
       inv TERMINAL0. ss. subst.
@@ -780,7 +485,7 @@ Proof.
         }
   - (* ite *)
     ii.
-    inversion LOCAL. exploit MemInv.sem_bot_inv; eauto. i.
+    inversion LOCAL. exploit SimPromises.sem_bot_inv; eauto. i.
     destruct lc_src, lc_tgt. ss. subst.
     splits; s; ii.
     { inv TERMINAL_TGT. }
@@ -788,7 +493,7 @@ Proof.
       esplits; eauto.
       - etrans.
         + apply Memory.max_timemap_spec; eauto. committac.
-        + apply Memory.sim_max_timemap; eauto. committac.
+        + apply sim_memory_max_timemap; eauto.
       - etrans.
         + apply Memory.max_timemap_spec; eauto. committac.
         + apply Memory.future_max_timemap; eauto.
@@ -822,7 +527,7 @@ Proof.
       }
   - (* dowhile *)
     ii.
-    inversion LOCAL. exploit MemInv.sem_bot_inv; eauto. i.
+    inversion LOCAL. exploit SimPromises.sem_bot_inv; eauto. i.
     destruct lc_src, lc_tgt. ss. subst.
     splits; s; ii.
     { inv TERMINAL_TGT. }
@@ -830,7 +535,7 @@ Proof.
       esplits; eauto.
       - etrans.
         + apply Memory.max_timemap_spec; eauto. committac.
-        + apply Memory.sim_max_timemap; eauto. committac.
+        + apply sim_memory_max_timemap; eauto.
       - etrans.
         + apply Memory.max_timemap_spec; eauto. committac.
         + apply Memory.future_max_timemap; eauto.
