src/opt/FulfillStep.v
@@ -17,8 +17,8 @@ Require Import Memory.
 Require Import MemoryFacts.
 Require Import Commit.
 Require Import Thread.
-Require Import Simulation.
-Require Import MemInv.
+
+Require Import SimMemory.
 
 Require Import Syntax.
 Require Import Semantics.
@@ -96,18 +96,20 @@ Lemma fulfill_write
       (SC1: Memory.closed_timemap sc1 mem1)
       (MEM1: Memory.closed mem1):
   exists released' mem2',
-    <<STEP: Local.write_step lc1 sc1 mem1 loc from to val releasedm released' ord lc2 sc2 mem2' Memory.promise_kind_lower>> /\
+    <<STEP: Local.write_step lc1 sc1 mem1 loc from to val releasedm released' ord lc2 sc2 mem2' (Memory.promise_kind_update from released)>> /\
     <<REL_LE: Capability.le released' released>> /\
-    <<MEM: Memory.sim mem1 mem2'>>.
+    <<MEM: sim_memory mem2' mem1>>.
 Proof.
   inv FULFILL.
   exploit remove_promise_remove; try exact REMOVE; eauto; try apply WF1.
   { repeat (try condtac; committac; try apply WF1). }
   i. des.
-  esplits; eauto. econs; eauto.
+  esplits; eauto.
   - econs; eauto.
-  - i. destruct ord; inv ORD; inv H.
-Qed.
+    + econs; eauto.
+    + i. destruct ord; inv ORD; inv H.
+  - admit. (* promise w/ same from => sim *)
+Admitted.
 
 Lemma promise_fulfill_write
       lc0 sc0 mem0 loc from to val releasedm released ord lc1 lc2 sc2 mem2 kind
@@ -123,7 +125,7 @@ Lemma promise_fulfill_write
   exists released' mem2',
     <<STEP: Local.write_step lc0 sc0 mem0 loc from to val releasedm released' ord lc2 sc2 mem2' kind>> /\
     <<REL_LE: Capability.le released' released>> /\
-    <<MEM: Memory.sim mem2 mem2'>>.
+    <<MEM: sim_memory mem2' mem2>>.
 Proof.
   exploit Local.promise_step_future; eauto. i. des.
   inv PROMISE. inv FULFILL.
@@ -131,7 +133,8 @@ Proof.
   { repeat (try condtac; committac; try apply WF2). }
   i. des.
   esplits; eauto.
-  refine (Local.step_write _ _ _ _ _); eauto.
-  econs; eauto.
-  admit. (* promise_kind + promise_lower <= promise_kind *)
+  - refine (Local.step_write _ _ _ _ _); eauto.
+    econs; eauto.
+    admit. (* promise_kind + promise_lower <= promise_kind *)
+  - admit. (* promise w/ same from => sim *)
 Admitted.
