src/opt/Merge.v
@@ -16,11 +16,13 @@ Require Import Memory.
 Require Import MemoryFacts.
 Require Import Commit.
 Require Import Thread.
-
 Require Import Configuration.
-Require Import Simulation.
+
+Require Import SimMemory.
+Require Import SimPromises.
+Require Import SimLocal.
 Require Import Compatibility.
-Require Import MemInv.
+Require Import Simulation.
 Require Import MergeStep.
 Require Import ReorderStep.
 
@@ -45,7 +47,7 @@ Proof.
     esplits; eauto.
     - etrans.
       + apply Memory.max_timemap_spec; eauto. committac.
-      + apply Memory.sim_max_timemap; eauto. committac.
+      + apply sim_memory_max_timemap; eauto.
     - etrans.
       + apply Memory.max_timemap_spec; eauto. committac.
       + apply Memory.future_max_timemap; eauto.
@@ -84,7 +86,7 @@ Proof.
     esplits; eauto.
     - etrans.
       + apply Memory.max_timemap_spec; eauto. committac.
-      + apply Memory.sim_max_timemap; eauto. committac.
+      + apply sim_memory_max_timemap; eauto.
     - etrans.
       + apply Memory.max_timemap_spec; eauto. committac.
       + apply Memory.future_max_timemap; eauto.
@@ -131,7 +133,7 @@ Proof.
     esplits; eauto.
     - etrans.
       + apply Memory.max_timemap_spec; eauto. committac.
-      + apply Memory.sim_max_timemap; eauto. committac.
+      + apply sim_memory_max_timemap; eauto.
     - etrans.
       + apply Memory.max_timemap_spec; eauto. committac.
       + apply Memory.future_max_timemap; eauto.
@@ -177,7 +179,7 @@ Proof.
     esplits; eauto.
     - etrans.
       + apply Memory.max_timemap_spec; eauto. committac.
-      + apply Memory.sim_max_timemap; eauto. committac.
+      + apply sim_memory_max_timemap; eauto.
     - etrans.
       + apply Memory.max_timemap_spec; eauto. committac.
       + apply Memory.future_max_timemap; eauto.
@@ -241,7 +243,7 @@ Proof.
     esplits; eauto.
     - etrans.
       + apply Memory.max_timemap_spec; eauto. committac.
-      + apply Memory.sim_max_timemap; eauto. committac.
+      + apply sim_memory_max_timemap; eauto.
     - etrans.
       + apply Memory.max_timemap_spec; eauto. committac.
       + apply Memory.future_max_timemap; eauto.
@@ -312,7 +314,7 @@ Proof.
     esplits; eauto.
     - etrans.
       + apply Memory.max_timemap_spec; eauto. committac.
-      + apply Memory.sim_max_timemap; eauto. committac.
+      + apply sim_memory_max_timemap; eauto.
     - etrans.
       + apply Memory.max_timemap_spec; eauto. committac.
       + apply Memory.future_max_timemap; eauto.
@@ -372,7 +374,7 @@ Proof.
     esplits; eauto.
     - etrans.
       + apply Memory.max_timemap_spec; eauto. committac.
-      + apply Memory.sim_max_timemap; eauto. committac.
+      + apply sim_memory_max_timemap; eauto.
     - etrans.
       + apply Memory.max_timemap_spec; eauto. committac.
       + apply Memory.future_max_timemap; eauto.
@@ -464,7 +466,7 @@ Proof.
     esplits; eauto.
     - etrans.
       + apply Memory.max_timemap_spec; eauto. committac.
-      + apply Memory.sim_max_timemap; eauto. committac.
+      + apply sim_memory_max_timemap; eauto.
     - etrans.
       + apply Memory.max_timemap_spec; eauto. committac.
       + apply Memory.future_max_timemap; eauto.
