src/opt/MergeMemory.v
@@ -15,11 +15,11 @@ Require Import Cell.
 Require Import Memory.
 Require Import Commit.
 Require Import Thread.
-
 Require Import Configuration.
-Require Import Simulation.
+
+Require Import SimPromises.
 Require Import Compatibility.
-Require Import MemInv.
+Require Import Simulation.
 
 Require Import Syntax.
 Require Import Semantics.
@@ -28,27 +28,34 @@ Set Implicit Arguments.
 
 
 Lemma remove_promise_remove_remove
-      promises1 loc ts1 ts2 ts3 val1 released1 val2 released2 promises4
-      mem1
-      (LE: Memory.le promises1 mem1)
-      (REMOVE: Memory.remove promises1 loc ts1 ts3 val2 released2 promises4):
-  exists promises2 mem2 promises3,
-    <<SPLIT: Memory.promise promises1 mem1 loc ts1 ts2 val1 released1 promises2 mem2 (Memory.promise_kind_split ts3)>> /\
-    <<REMOVE1: Memory.remove promises2 loc ts1 ts2 val1 released1 promises3>> /\
-    <<REMOVE2: Memory.remove promises3 loc ts2 ts3 val2 released2 promises4>>.
+      loc ts1 ts2 ts3 val2 released2
+      promises0 mem0
+      promises4
+      (LE: Memory.le promises0 mem0)
+      (REMOVE: Memory.remove promises0 loc ts1 ts3 val2 released2 promises4):
+  exists promises1 mem1 promises3,
+    <<STEP1: Memory.promise promises0 mem0 loc ts2 ts3 val2 released2 promises1 mem1 (Memory.promise_kind_update ts1 released2)>> /\
+    <<STEPS:
+      forall val1 released1,
+      exists promises2 mem2,
+        <<STEP2: Memory.promise promises1 mem1 loc ts1 ts2 val1 released1 promises2 mem2 Memory.promise_kind_add>> /\
+        <<STEP3: Memory.remove promises2 loc ts1 ts2 val1 released1 promises3>> /\
+        <<STEP4: Memory.remove promises3 loc ts2 ts3 val2 released2 promises4>>>>.
 Proof.
 Admitted.
 
 Lemma promise_remove_promise_remove_promise_remove
-      promises1 loc ts1 ts2 ts3 val1 released1 val2 released2 promises4 promises5
-      mem1 mem4
-      (LE: Memory.le promises1 mem1)
-      (PROMISE: Memory.promise promises1 mem1 loc ts1 ts3 val2 released2 promises4 mem4 Memory.promise_kind_add)
+      loc ts1 ts2 ts3 val2 val1 released1 released2
+      promises0 mem0
+      mem4 promises4
+      promises5
+      (LE: Memory.le promises0 mem0)
+      (PROMISE: Memory.promise promises0 mem0 loc ts1 ts3 val2 released2 promises4 mem4 Memory.promise_kind_add)
       (REMOVE: Memory.remove promises4 loc ts1 ts3 val2 released2 promises5):
-  exists promises2 mem2 promises3 promises4 mem4,
-    <<PROMISE1: Memory.promise promises1 mem1 loc ts1 ts2 val1 released1 promises2 mem2 Memory.promise_kind_add>> /\
-    <<REMOVE1: Memory.remove promises2 loc ts1 ts2 val1 released1 promises3>> /\
-    <<PROMISE2: Memory.promise promises3 mem2 loc ts2 ts3 val2 released2 promises4 mem4 Memory.promise_kind_add>> /\
-    <<REMOVE2: Memory.remove promises4 loc ts2 ts3 val2 released2 promises5>>.
+  exists promises1 promises2 promises3 mem1 mem3,
+    <<STEP1: Memory.promise promises0 mem0 loc ts1 ts2 val1 released1 promises1 mem1 Memory.promise_kind_add>> /\
+    <<STEP2: Memory.remove promises1 loc ts1 ts2 val1 released1 promises2>> /\
+    <<STEP3: Memory.promise promises2 mem1 loc ts2 ts3 val2 released2 promises3 mem3 Memory.promise_kind_add>> /\
+    <<STEP4: Memory.remove promises3 loc ts2 ts3 val2 released2 promises4>>.
 Proof.
 Admitted.
