src/opt/MergeStep.v
@@ -13,14 +13,18 @@ Require Import Time.
 Require Import View.
 Require Import Cell.
 Require Import Memory.
+Require Import MemoryFacts.
 Require Import Commit.
 Require Import Thread.
-
 Require Import Configuration.
-Require Import Simulation.
-Require Import Compatibility.
-Require Import MemInv.
 Require Import Progress.
+
+Require Import FulfillStep.
+Require Import SimMemory.
+Require Import SimPromises.
+Require Import SimLocal.
+Require Import Compatibility.
+Require Import Simulation.
 
 Require MergeCommit.
 Require MergeMemory.
@@ -113,38 +117,46 @@ Lemma merge_write_write_relaxed
       (TS12: Time.lt ts1 ts2)
       (TS23: Time.lt ts2 ts3)
       (STEP: Local.write_step lc0 sc0 mem0 loc ts1 ts3 val2 released0 released2 ord lc3 sc3 mem3 kind):
-  exists lc1' lc2' lc3' sc2' sc3' mem2' mem3' released1' released2',
-    <<STEP1: Local.promise_step lc0 mem0 loc ts1 ts3 val2 released2 lc1' mem3 kind>> /\
-    <<STEP2: Local.write_step lc1' sc0 mem3 loc ts1 ts2 val1 released0 released1' ord lc2' sc2' mem2' (Memory.promise_kind_split ts3)>> /\
-    <<STEP3: Local.write_step lc2' sc2' mem2' loc ts2 ts3 val2 released1' released2' ord lc3' sc3' mem3' Memory.promise_kind_lower>> /\
+  exists lc1' lc2' lc3' sc2' sc3' mem1' mem2' mem3' released1' released2',
+    <<STEP1: Local.promise_step lc0 mem0 loc ts2 ts3 val2 released2 lc1' mem1' kind>> /\
+    <<STEP2: Local.write_step lc1' sc0 mem1' loc ts1 ts2 val1 released0 released1' ord lc2' sc2' mem2' Memory.promise_kind_add>> /\
+    <<STEP3: Local.write_step lc2' sc2' mem2' loc ts2 ts3 val2 released1' released2' ord lc3' sc3' mem3' (Memory.promise_kind_update ts2 released2)>> /\
     <<REL3: Capability.le released2' released2>> /\
     <<LOCAL3: sim_local lc3' lc3>> /\
     <<SC3: TimeMap.le sc3' sc3>> /\
-    <<MEM3: Memory.sim mem3 mem3'>>.
+    <<MEM3: sim_memory mem3' mem3>>.
 Proof.
-  exploit Local.write_step_future; eauto. i. des.
-  inv STEP. inv WRITE.
-  exploit Memory.promise_future0 ; try apply PROMISE; try apply WF0; eauto; try by committac. i. des.
-  exploit MergeMemory.remove_promise_remove_remove; try apply REMOVE; eauto. i. des.
+  exploit write_promise_fulfill; eauto. i. des.
+  exploit Local.promise_step_future; eauto. i. des.
+  exploit fulfill_step_future; try exact STEP2; try exact WF2; eauto; try by committac. i. des.
+  inv STEP1. inv STEP2.
+  exploit MergeMemory.remove_promise_remove_remove; try apply WF2; eauto. i. des.
+  exploit STEPS; eauto. i. des.
+  hexploit remove_promise_remove; try eexact STEP4.
+  { admit. (* promise_future *) }
+  { admit. }
+  { repeat (try condtac; aggrtac; try apply WF0). }
+  { admit. }
+  { eexact TS23. }
+  i. des.
   esplits.
-  - econs; eauto.
+  - econs.
+    + eapply promise_promise_promise; eauto.
+    + admit. (* closed capability *)
   - econs; eauto.
     + admit. (* writable *)
     + econs; eauto.
     + i. destruct ord; inv ORD; inv H.
   - econs; eauto.
     + admit. (* writable *)
-    + instantiate (1 := mem2).
-      econs; eauto.
-      * admit. (* promsie *)
-      * unfold Local.commit at 1 3 4.
-        admit. (* remove *)
+    + econs; eauto.
     + i. destruct ord; inv ORD; inv H.
   - repeat (try condtac; aggrtac; try apply WF0).
   - s. econs; ss.
-    eapply MergeCommit.write_write_commit; eauto. apply WF0.
+    + eapply MergeCommit.write_write_commit; eauto. apply WF0.
+    + apply SimPromises.sem_bot.
   - eapply MergeCommit.write_write_sc; eauto.
-  - inv SPLIT. econs 2; eauto. econs 1. eauto.
+  - admit. (* sim_memory *)
 Admitted.
 
 Lemma merge_write_write_add
@@ -165,7 +177,7 @@ Lemma merge_write_write_add
     <<REL2: Capability.le released2' released2>> /\
     <<LOCAL2: sim_local lc2' lc2>> /\
     <<SC2: TimeMap.le sc2' sc2>> /\
-    <<MEM2: Memory.sim mem2 mem2'>>.
+    <<MEM2: sim_memory mem2' mem2>>.
 Proof.
 Admitted.
 
@@ -182,17 +194,17 @@ Lemma merge_write_write
       (TS23: Time.lt ts2 ts3)
       (STEP: Local.write_step lc0 sc0 mem0 loc ts1 ts3 val2 released0 released2 ord lc3 sc3 mem3 kind):
   exists lc1' lc2' lc3' sc2' sc3' mem1' mem2' mem3' released1' released2' kind2 kind3,
-    <<STEP1: Local.promise_step lc0 mem0 loc ts1 ts3 val2 released2 lc1' mem1' kind \/ (lc0, mem0) = (lc1', mem1')>> /\
+    <<STEP1: Local.promise_step lc0 mem0 loc ts2 ts3 val2 released2 lc1' mem1' kind \/ (lc0, mem0) = (lc1', mem1')>> /\
     <<STEP2: Local.write_step lc1' sc0 mem1' loc ts1 ts2 val1 released0 released1' ord lc2' sc2' mem2' kind2>> /\
     <<STEP3: Local.write_step lc2' sc2' mem2' loc ts2 ts3 val2 released1' released2' ord lc3' sc3' mem3' kind3>> /\
     <<REL3: Capability.le released2' released2>> /\
     <<LOCAL3: sim_local lc3' lc3>> /\
     <<SC3: TimeMap.le sc3' sc3>> /\
-    <<MEM3: Memory.sim mem3 mem3'>>.
+    <<MEM3: sim_memory mem3' mem3>>.
 Proof.
   destruct (Ordering.le ord Ordering.relaxed) eqn:ORD.
   - exploit merge_write_write_relaxed; try apply TS12; eauto. i. des.
-    esplits; try apply STEP2; eauto.
+    esplits; try exact STEP2; eauto.
   - assert (kind = Memory.promise_kind_add).
     { inv STEP. eapply RELEASE. by destruct ord; inv ORD. }
     subst. exploit merge_write_write_add; try apply TS12; eauto. i. des.
@@ -212,13 +224,13 @@ Lemma merge_write_write_bot
       (TS23: Time.lt ts2 ts3)
       (STEP: Local.write_step lc0 sc0 mem0 loc ts1 ts3 val2 released0 released2 ord lc3 sc3 mem3 kind):
   exists lc1' lc2' lc3' sc2' sc3' mem1' mem2' mem3' released1' released2' kind2 kind3,
-    <<STEP1: Local.promise_step lc0 mem0 loc ts1 ts3 val2 released2 lc1' mem1' kind \/ (lc0, mem0) = (lc1', mem1')>> /\
+    <<STEP1: Local.promise_step lc0 mem0 loc ts2 ts3 val2 released2 lc1' mem1' kind \/ (lc0, mem0) = (lc1', mem1')>> /\
     <<STEP2: Local.write_step lc1' sc0 mem1' loc ts1 ts2 val1 released0 released1' ord lc2' sc2' mem2' kind2>> /\
     <<STEP3: Local.write_step lc2' sc2' mem2' loc ts2 ts3 val2 Capability.bot released2' ord lc3' sc3' mem3' kind3>> /\
     <<REL3: Capability.le released2' released2>> /\
     <<LOCAL3: sim_local lc3' lc3>> /\
     <<SC3: TimeMap.le sc3' sc3>> /\
-    <<MEM3: Memory.sim mem3 mem3'>>.
+    <<MEM3: sim_memory mem3' mem3>>.
 Proof.
   exploit merge_write_write; try apply TS12; eauto. i. des.
   - exploit Local.promise_step_future; eauto. i. des.
@@ -240,10 +252,10 @@ Lemma merge_fence_fence
       lc2 sc2
       (WF0: Local.wf lc0 mem0)
       (MEM0: Memory.closed mem0)
-      (STEP: Local.fence_step lc0 sc0 mem0 ordr ordw lc2 sc2):
+      (STEP: Local.fence_step lc0 sc0 ordr ordw lc2 sc2):
   exists lc1 lc2' sc1' sc2',
-    <<STEP1: Local.fence_step lc0 sc0 mem0 ordr ordw lc1 sc1'>> /\
-    <<STEP2: Local.fence_step lc1 sc1' mem0 ordr ordw lc2' sc2'>> /\
+    <<STEP1: Local.fence_step lc0 sc0 ordr ordw lc1 sc1'>> /\
+    <<STEP2: Local.fence_step lc1 sc1' ordr ordw lc2' sc2'>> /\
     <<LOCAL: sim_local lc2' lc2>> /\
     <<SC2: TimeMap.le sc2' sc2>>.
 Proof.
@@ -259,6 +271,7 @@ Proof.
       apply MergeCommit.read_fence_read_fence_commit; eauto. apply WF0.
     + eapply MergeCommit.write_fence_write_fence_commit; eauto.
       eapply CommitFacts.read_fence_future; apply WF0.
+    + apply SimPromises.sem_bot.
   - s. etrans; [etrans|].
     + apply CommitFacts.write_fence_sc_mon; [|refl|refl].
       eapply ReorderCommit.read_fence_write_fence_commit.
