src/opt/SimLocal.v
@@ -1,0 +1,352 @@
+Require Import RelationClasses.
+Require Import Basics.
+Require Import Bool.
+Require Import List.
+
+Require Import sflib.
+Require Import paco.
+Require Import respectful9.
+
+Require Import Axioms.
+Require Import Basic.
+Require Import Event.
+Require Import Time.
+Require Import Language.
+Require Import View.
+Require Import Cell.
+Require Import Memory.
+Require Import Commit.
+Require Import Thread.
+Require Import Configuration.
+
+Require Import FulfillStep.
+Require Import SimMemory.
+Require Import SimPromises.
+
+Require Import Syntax.
+Require Import Semantics.
+
+Set Implicit Arguments.
+
+
+Inductive sim_local (lc_src lc_tgt:Local.t): Prop :=
+| sim_local_intro
+    (COMMIT: Commit.le lc_src.(Local.commit) lc_tgt.(Local.commit))
+    (PROMISES: SimPromises.sem SimPromises.bot lc_src.(Local.promises) lc_tgt.(Local.promises))
+.
+
+Program Instance sim_local_PreOrder: PreOrder sim_local.
+Next Obligation.
+  econs; try refl. apply SimPromises.sem_bot.
+Qed.
+Next Obligation.
+  ii. inv H. inv H0. econs; try etrans; eauto.
+  apply SimPromises.sem_bot_inv in PROMISES; auto.
+  apply SimPromises.sem_bot_inv in PROMISES0; auto.
+  rewrite PROMISES, PROMISES0. apply SimPromises.sem_bot.
+Qed.
+
+Lemma sim_local_cell_bot
+      loc lc_src lc_tgt
+      (SIM: sim_local lc_src lc_tgt)
+      (BOT: lc_tgt.(Local.promises) loc = Cell.bot):
+  lc_src.(Local.promises) loc = Cell.bot.
+Proof.
+  inv SIM. eapply SimPromises.sem_bot_inv in PROMISES; auto. rewrite PROMISES. auto.
+Qed.
+
+Lemma sim_local_memory_bot
+      lc_src lc_tgt
+      (SIM: sim_local lc_src lc_tgt)
+      (BOT: lc_tgt.(Local.promises) = Memory.bot):
+  lc_src.(Local.promises) = Memory.bot.
+Proof.
+  inv SIM. eapply SimPromises.sem_bot_inv in PROMISES; auto. rewrite PROMISES. auto.
+Qed.
+
+Lemma sim_local_future
+      inv
+      lc_src mem1_src mem2_src
+      lc_tgt mem1_tgt
+      (INV1: SimPromises.sem inv lc_src.(Local.promises) lc_tgt.(Local.promises))
+      (MEM1: sim_memory mem1_src mem1_tgt)
+      (FUTURE_SRC: Memory.future mem1_src mem2_src)
+      (WF1_SRC: Local.wf lc_src mem1_src)
+      (WF1_TGT: Local.wf lc_tgt mem1_tgt)
+      (WF2_SRC: Local.wf lc_src mem2_src)
+      (MEM1_SRC: Memory.closed mem1_src)
+      (MEM1_TGT: Memory.closed mem1_tgt):
+  exists mem2_tgt,
+    <<MEM2: sim_memory mem2_src mem2_tgt>> /\
+    <<FUTURE_TGT: Memory.future mem1_tgt mem2_tgt>> /\
+    <<WF2_TGT: Local.wf lc_tgt mem2_tgt>> /\
+    <<MEM2_TGT: Memory.closed mem2_tgt>>.
+Proof.
+  exploit SimPromises.future; eauto.
+  { apply WF1_SRC. }
+  { apply WF1_TGT. }
+  { apply WF2_SRC. }
+  i. des.
+  esplits; eauto.
+  econs; eauto.
+  - apply WF1_TGT.
+  - eapply Commit.future_closed; eauto. apply WF1_TGT.
+Qed.
+
+Lemma promise_future
+      promises1 mem1 loc from to val released promises2 mem2 kind
+      (PROMISE: Memory.promise promises1 mem1 loc from to val released promises2 mem2 kind):
+  Memory.future mem1 mem2.
+Proof.
+  econs 2; eauto. inv PROMISE.
+  - econs 1. eauto.
+  - econs 2. eauto.
+Qed.
+
+Lemma sim_local_promise
+      lc1_src mem1_src
+      lc1_tgt mem1_tgt
+      lc2_tgt mem2_tgt
+      loc from to val released kind
+      (STEP_TGT: Local.promise_step lc1_tgt mem1_tgt loc from to val released lc2_tgt mem2_tgt kind)
+      (LOCAL1: sim_local lc1_src lc1_tgt)
+      (MEM1: sim_memory mem1_src mem1_tgt)
+      (WF1_SRC: Local.wf lc1_src mem1_src)
+      (WF1_TGT: Local.wf lc1_tgt mem1_tgt)
+      (MEM1_SRC: Memory.closed mem1_src)
+      (MEM1_TGT: Memory.closed mem1_tgt):
+  exists lc2_src mem2_src,
+    <<STEP_SRC: Local.promise_step lc1_src mem1_src loc from to val released lc2_src mem2_src kind>> /\
+    <<LOCAL2: sim_local lc2_src lc2_tgt>> /\
+    <<MEM2: sim_memory mem2_src mem2_tgt>>.
+Proof.
+  inv LOCAL1. inv STEP_TGT.
+  exploit SimPromises.promise; eauto.
+  { apply WF1_SRC. }
+  { apply WF1_TGT. }
+  i. des.
+  exploit sim_memory_closed_capability; eauto. i.
+  exploit Memory.promise_future; try apply PROMISE_SRC; eauto.
+  { apply WF1_SRC. }
+  i. des.
+  esplits; eauto.
+  - econs; eauto.
+  - econs; eauto.
+Qed.
+
+Lemma sim_local_read
+      lc1_src mem1_src
+      lc1_tgt mem1_tgt
+      lc2_tgt
+      loc ts val released_tgt ord_src ord_tgt
+      (STEP_TGT: Local.read_step lc1_tgt mem1_tgt loc ts val released_tgt ord_tgt lc2_tgt)
+      (LOCAL1: sim_local lc1_src lc1_tgt)
+      (MEM1: sim_memory mem1_src mem1_tgt)
+      (WF1_SRC: Local.wf lc1_src mem1_src)
+      (WF1_TGT: Local.wf lc1_tgt mem1_tgt)
+      (MEM1_SRC: Memory.closed mem1_src)
+      (MEM1_TGT: Memory.closed mem1_tgt)
+      (ORD: Ordering.le ord_src ord_tgt):
+  exists released_src lc2_src,
+    <<REL: Capability.le released_src released_tgt>> /\
+    <<STEP_SRC: Local.read_step lc1_src mem1_src loc ts val released_src ord_src lc2_src>> /\
+    <<LOCAL2: sim_local lc2_src lc2_tgt>>.
+Proof.
+  inv LOCAL1. inv STEP_TGT.
+  exploit sim_memory_get; try apply MEM1; eauto. i. des.
+  esplits; eauto.
+  - econs; eauto. eapply CommitFacts.readable_mon; eauto.
+  - econs; eauto. s. apply CommitFacts.read_commit_mon; auto.
+    + apply WF1_TGT.
+    + eapply MEM1_TGT. eauto.
+Qed.
+
+Lemma sim_local_fulfill
+      lc1_src sc1_src mem1_src
+      lc1_tgt sc1_tgt mem1_tgt
+      lc2_tgt sc2_tgt
+      loc from to val releasedm_src releasedm_tgt released ord
+      (RELM_LE: Capability.le releasedm_src releasedm_tgt)
+      (RELM_WF: Capability.wf releasedm_src)
+      (RELM_CLOSED: Memory.closed_capability releasedm_src mem1_src)
+      (WF_RELM_TGT: Capability.wf releasedm_tgt)
+      (STEP_TGT: fulfill_step lc1_tgt sc1_tgt loc from to val releasedm_tgt released ord lc2_tgt sc2_tgt)
+      (LOCAL1: sim_local lc1_src lc1_tgt)
+      (SC1: TimeMap.le sc1_src sc1_tgt)
+      (MEM1: sim_memory mem1_src mem1_tgt)
+      (WF1_SRC: Local.wf lc1_src mem1_src)
+      (WF1_TGT: Local.wf lc1_tgt mem1_tgt)
+      (SC1_SRC: Memory.closed_timemap sc1_src mem1_src)
+      (SC1_TGT: Memory.closed_timemap sc1_tgt mem1_tgt)
+      (MEM1_SRC: Memory.closed mem1_src)
+      (MEM1_TGT: Memory.closed mem1_tgt):
+  exists lc2_src sc2_src,
+    <<STEP_SRC: fulfill_step lc1_src sc1_src loc from to val releasedm_src released ord lc2_src sc2_src>> /\
+    <<LOCAL2: sim_local lc2_src lc2_tgt>> /\
+    <<SC2: TimeMap.le sc2_src sc2_tgt>>.
+Proof.
+  inv STEP_TGT.
+  assert (RELT_LE:
+   Capability.le
+     (Capability.join releasedm_src
+        (Commit.rel
+           (Commit.write_commit (Local.commit lc1_src) sc1_src loc to
+              ord) loc))
+     (Capability.join releasedm_tgt
+        (Commit.rel
+           (Commit.write_commit (Local.commit lc1_tgt) sc1_tgt loc to
+              ord) loc))).
+  { committac.
+    - etrans; eauto. committac.
+    - rewrite <- Capability.join_r.
+      rewrite <- Capability.join_l.
+      apply LOCAL1.
+    - condtac; committac; try apply WF1_TGT.
+      + rewrite <- Capability.join_r.
+        rewrite <- Capability.join_r.
+        rewrite <- Capability.join_l.
+        rewrite <- Capability.join_l.
+        apply LOCAL1.
+      + condtac; committac.
+      + etrans; [|apply TimeMap.join_r].
+        etrans; [|apply TimeMap.join_r].
+        etrans; [|apply TimeMap.join_l].
+        etrans; [|apply TimeMap.join_r].
+        unfold TimeMap.singleton, LocFun.add. condtac; [refl|congr].
+      + condtac; committac.
+        rewrite <- Capability.join_r.
+        rewrite <- Capability.join_r.
+        rewrite <- Capability.join_r.
+        econs; try refl. ss.
+  }
+  assert (RELT_WF:
+   Capability.wf
+     (Capability.join releasedm_src
+        (Commit.rel
+           (Commit.write_commit (Local.commit lc1_src) sc1_src loc to
+              ord) loc))).
+  { repeat (try condtac; committac; try apply WF1_SRC). }
+  exploit SimPromises.remove; try exact REMOVE;
+    try exact MEM1; try apply LOCAL1; eauto.
+  { apply WF1_SRC. }
+  { apply WF1_TGT. }
+  i. des. esplits.
+  - econs; eauto.
+    + etrans; eauto.
+    + eapply CommitFacts.writable_mon; eauto. apply LOCAL1. refl.
+  - econs; eauto. s. apply CommitFacts.write_commit_mon; auto.
+    + apply LOCAL1.
+    + apply WF1_TGT.
+    + refl.
+  - apply CommitFacts.write_sc_mon; auto. refl.
+Qed.
+
+Lemma sim_local_write
+      lc1_src sc1_src mem1_src
+      lc1_tgt sc1_tgt mem1_tgt
+      lc2_tgt sc2_tgt mem2_tgt
+      loc from to val releasedm_src releasedm_tgt released_tgt ord kind
+      (RELM_LE: Capability.le releasedm_src releasedm_tgt)
+      (RELM_SRC_WF: Capability.wf releasedm_src)
+      (RELM_SRC_CLOSED: Memory.closed_capability releasedm_src mem1_src)
+      (RELM_TGT_WF: Capability.wf releasedm_tgt)
+      (RELM_TGT_CLOSED: Memory.closed_capability releasedm_tgt mem1_tgt)
+      (STEP_TGT: Local.write_step lc1_tgt sc1_tgt mem1_tgt loc from to val releasedm_tgt released_tgt ord lc2_tgt sc2_tgt mem2_tgt kind)
+      (LOCAL1: sim_local lc1_src lc1_tgt)
+      (SC1: TimeMap.le sc1_src sc1_tgt)
+      (MEM1: sim_memory mem1_src mem1_tgt)
+      (WF1_SRC: Local.wf lc1_src mem1_src)
+      (WF1_TGT: Local.wf lc1_tgt mem1_tgt)
+      (SC1_SRC: Memory.closed_timemap sc1_src mem1_src)
+      (SC1_TGT: Memory.closed_timemap sc1_tgt mem1_tgt)
+      (MEM1_SRC: Memory.closed mem1_src)
+      (MEM1_TGT: Memory.closed mem1_tgt):
+  exists released_src lc2_src sc2_src mem2_src,
+    <<STEP_SRC: Local.write_step lc1_src sc1_src mem1_src loc from to val releasedm_src released_src ord lc2_src sc2_src mem2_src kind>> /\
+    <<REL2: Capability.le released_src released_tgt>> /\
+    <<LOCAL2: sim_local lc2_src lc2_tgt>> /\
+    <<SC2: TimeMap.le sc2_src sc2_tgt>> /\
+    <<MEM2: sim_memory mem2_src mem2_tgt>>.
+Proof.
+  exploit write_promise_fulfill; eauto. i. des.
+  exploit Local.promise_step_future; eauto. i. des.
+  exploit sim_local_promise; eauto. i. des.
+  exploit Local.promise_step_future; eauto. i. des.
+  exploit sim_local_fulfill; try apply STEP2;
+    try apply LOCAL2; try apply MEM2; eauto.
+  { eapply Memory.future_closed_capability; eauto. }
+  i. des.
+  exploit promise_fulfill_write; try exact STEP_SRC; try exact STEP_SRC0; eauto.
+  { i. exploit ORD; eauto. i. des.
+    splits; auto. eapply sim_local_cell_bot; eauto.
+  }
+  i. des. esplits; eauto. etrans; eauto.
+Qed.
+
+Lemma sim_local_update
+      lc1_src sc1_src mem1_src
+      lc1_tgt sc1_tgt mem1_tgt
+      lc2_tgt
+      lc3_tgt sc3_tgt mem3_tgt
+      loc ts1 val1 released1_tgt ord1_src ord1_tgt
+      from2 to2 val2 released2_tgt ord2 kind
+      (STEP1_TGT: Local.read_step lc1_tgt mem1_tgt loc ts1 val1 released1_tgt ord1_tgt lc2_tgt)
+      (STEP2_TGT: Local.write_step lc2_tgt sc1_tgt mem1_tgt loc from2 to2 val2 released1_tgt released2_tgt ord2 lc3_tgt sc3_tgt mem3_tgt kind)
+      (LOCAL1: sim_local lc1_src lc1_tgt)
+      (SC1: TimeMap.le sc1_src sc1_tgt)
+      (MEM1: sim_memory mem1_src mem1_tgt)
+      (WF1_SRC: Local.wf lc1_src mem1_src)
+      (WF1_TGT: Local.wf lc1_tgt mem1_tgt)
+      (SC1_SRC: Memory.closed_timemap sc1_src mem1_src)
+      (SC1_TGT: Memory.closed_timemap sc1_tgt mem1_tgt)
+      (MEM1_SRC: Memory.closed mem1_src)
+      (MEM1_TGT: Memory.closed mem1_tgt)
+      (ORD: Ordering.le ord1_src ord1_tgt):
+  exists released1_src released2_src lc2_src lc3_src sc3_src mem3_src,
+    <<REL1: Capability.le released1_src released1_tgt>> /\
+    <<REL2: Capability.le released2_src released2_tgt>> /\
+    <<STEP1_SRC: Local.read_step lc1_src mem1_src loc ts1 val1 released1_src ord1_src lc2_src>> /\
+    <<STEP2_SRC: Local.write_step lc2_src sc1_src mem1_src loc from2 to2 val2 released1_src released2_src ord2 lc3_src sc3_src mem3_src kind>> /\
+    <<LOCAL3: sim_local lc3_src lc3_tgt>> /\
+    <<SC3: TimeMap.le sc3_src sc3_tgt>> /\
+    <<MEM3: sim_memory mem3_src mem3_tgt>>.
+Proof.
+  exploit Local.read_step_future; eauto. i. des.
+  exploit sim_local_read; eauto. i. des.
+  exploit Local.read_step_future; eauto. i. des.
+  exploit sim_local_write; eauto. i. des.
+  esplits; eauto.
+Qed.
+
+Lemma sim_local_fence
+      lc1_src sc1_src mem1_src
+      lc1_tgt sc1_tgt mem1_tgt
+      lc2_tgt sc2_tgt
+      ordr_src ordw_src
+      ordr_tgt ordw_tgt
+      (STEP_TGT: Local.fence_step lc1_tgt sc1_tgt ordr_tgt ordw_tgt lc2_tgt sc2_tgt)
+      (LOCAL1: sim_local lc1_src lc1_tgt)
+      (SC1: TimeMap.le sc1_src sc1_tgt)
+      (MEM1: sim_memory mem1_src mem1_tgt)
+      (WF1_SRC: Local.wf lc1_src mem1_src)
+      (WF1_TGT: Local.wf lc1_tgt mem1_tgt)
+      (ORDR: Ordering.le ordr_src ordr_tgt)
+      (ORDW: Ordering.le ordw_src ordw_tgt):
+  exists lc2_src sc2_src,
+    <<STEP_SRC: Local.fence_step lc1_src sc1_src ordr_src ordw_src lc2_src sc2_src>> /\
+    <<LOCAL2: sim_local lc2_src lc2_tgt>> /\
+    <<SC2: TimeMap.le sc2_src sc2_tgt>>.
+Proof.
+  inv STEP_TGT. esplits; eauto.
+  - econs; eauto. i. eapply sim_local_memory_bot; eauto.
+    apply RELEASE. etrans; eauto.
+  - econs; try apply LOCAL1. s.
+    apply CommitFacts.write_fence_commit_mon; auto; try refl.
+    apply CommitFacts.read_fence_commit_mon; auto; try refl.
+    + apply LOCAL1.
+    + apply WF1_TGT.
+  - apply CommitFacts.write_fence_sc_mon; auto; try refl.
+    apply CommitFacts.read_fence_commit_mon; auto; try refl.
+    + apply LOCAL1.
+    + apply WF1_TGT.
+Qed.
