src/opt/SimMemory.v
@@ -1,0 +1,134 @@
+Require Import RelationClasses.
+Require Import Basics.
+Require Import Bool.
+Require Import List.
+
+Require Import sflib.
+Require Import paco.
+Require Import respectful5.
+
+Require Import Axioms.
+Require Import Basic.
+Require Import Event.
+Require Import DenseOrder.
+Require Import Time.
+Require Import Language.
+Require Import View.
+Require Import Cell.
+Require Import Memory.
+Require Import MemoryFacts.
+Require Import Commit.
+Require Import Thread.
+Require Import Configuration.
+
+Set Implicit Arguments.
+
+
+Inductive covered (loc:Loc.t) (ts:Time.t) (mem:Memory.t): Prop :=
+| covered_intro
+    from to msg
+    (GET: Memory.get loc to mem = Some (from, msg))
+    (ITV: Interval.mem (from, to) ts)
+.
+
+Inductive sim_memory (mem_src mem_tgt:Memory.t): Prop :=
+| sim_memory_intro
+    (COVER: forall loc ts, covered loc ts mem_src <-> covered loc ts mem_tgt)
+    (MSG: forall loc from_tgt to val released_tgt
+            (GET: Memory.get loc to mem_tgt = Some (from_tgt, Message.mk val released_tgt)),
+        exists from_src released_src,
+          <<GET: Memory.get loc to mem_src = Some (from_src, Message.mk val released_src)>> /\
+          <<RELEASED: Capability.le released_src released_tgt>>)
+.
+
+Program Instance sim_memory_PreOrder: PreOrder sim_memory.
+Next Obligation.
+  econs; try refl. i. esplits; eauto. refl.
+Qed.
+Next Obligation.
+  ii. inv H. inv H0. econs; try etrans; eauto. i.
+  exploit MSG0; eauto. i. des.
+  exploit MSG; eauto. i. des.
+  esplits; eauto. etrans; eauto.
+Qed.
+
+
+Lemma sim_memory_get
+      loc from_tgt to val released_tgt mem_src mem_tgt
+      (SIM: sim_memory mem_src mem_tgt)
+      (GET: Memory.get loc to mem_tgt = Some (from_tgt, Message.mk val released_tgt)):
+  exists from_src released_src,
+    <<GET: Memory.get loc to mem_src = Some (from_src, Message.mk val released_src)>> /\
+    <<RELEASED: Capability.le released_src released_tgt>>.
+Proof.
+  eapply SIM. eauto.
+Qed.
+
+Lemma sim_memory_max_timemap
+      mem_src mem_tgt
+      (CLOSED_SRC: Memory.closed mem_src)
+      (CLOSED_TGT: Memory.closed mem_tgt)
+      (SIM: sim_memory mem_src mem_tgt):
+  TimeMap.le (Memory.max_timemap mem_src) (Memory.max_timemap mem_tgt).
+Proof.
+Admitted.
+
+Lemma sim_memory_add
+      mem1_src mem1_tgt
+      mem2_src mem2_tgt
+      loc from to val released
+      (SRC: Memory.add mem1_src loc from to val released mem2_src)
+      (TGT: Memory.add mem1_tgt loc from to val released mem2_tgt)
+      (SIM: sim_memory mem1_src mem1_tgt):
+  sim_memory mem2_src mem2_tgt.
+Proof.
+Admitted.
+
+Lemma sim_memory_update
+      mem1_src mem1_tgt
+      mem2_src mem2_tgt
+      loc from1 from2 to val released1 released2
+      (SRC: Memory.update mem1_src loc from1 from2 to val released1 released2 mem2_src)
+      (TGT: Memory.update mem1_tgt loc from1 from2 to val released1 released2 mem2_tgt)
+      (SIM: sim_memory mem1_src mem1_tgt):
+  sim_memory mem2_src mem2_tgt.
+Proof.
+Admitted.
+
+Lemma sim_memory_promise
+      loc from to val released kind
+      promises1_src mem1_src promises2_src mem2_src
+      promises1_tgt mem1_tgt promises2_tgt mem2_tgt
+      (PROMISE_SRC: Memory.promise promises1_src mem1_src loc from to val released promises2_src mem2_src kind)
+      (PROMISE_TGT: Memory.promise promises1_tgt mem1_tgt loc from to val released promises2_tgt mem2_tgt kind)
+      (SIM: sim_memory mem1_src mem1_tgt):
+  sim_memory mem2_src mem2_tgt.
+Proof.
+  inv PROMISE_SRC; inv PROMISE_TGT.
+  - eapply sim_memory_add; eauto.
+  - eapply sim_memory_update; eauto.
+Qed.
+
+Lemma sim_memory_closed_timemap
+      mem_src mem_tgt
+      tm
+      (SIM: sim_memory mem_src mem_tgt)
+      (TGT: Memory.closed_timemap tm mem_tgt):
+  Memory.closed_timemap tm mem_src.
+Proof.
+  ii. exploit TGT; eauto. i. des.
+  exploit sim_memory_get; eauto. i. des. eauto.
+Qed.
+
+Lemma sim_memory_closed_capability
+      mem_src mem_tgt
+      capability
+      (SIM: sim_memory mem_src mem_tgt)
+      (TGT: Memory.closed_capability capability mem_tgt):
+  Memory.closed_capability capability mem_src.
+Proof.
+  econs.
+  - eapply sim_memory_closed_timemap; eauto. apply TGT.
+  - eapply sim_memory_closed_timemap; eauto. apply TGT.
+  - eapply sim_memory_closed_timemap; eauto. apply TGT.
+Qed.
